Move Store type/fn out.

src/dafny/beacon/forkchoice/ForkChoiceHelpers.dfy
@@ -73,7 +73,8 @@ module ForkChoiceHelpers {
 
     /**
      *  A valid pending attestation. 
-     *  @param  a       A pending attestattion.
+     *  @param  a       A pending attestation.
+     *
      *  @param  store   A store.
      *  @param  links   A sequence of votes.
      */
@@ -101,23 +102,23 @@ module ForkChoiceHelpers {
      *
      *  @param  store   A store.
      */
-    predicate isClosedUnderParent(store: Store) 
-    {
-        forall k {:trigger store.blocks[k]}:: k in store.blocks.Keys && store.blocks[k].slot > 0 ==>
-            store.blocks[k].parent_root in store.blocks.Keys
-    }
+    // predicate isClosedUnderParent(store: Store) 
+    // {
+    //     forall k {:trigger store.blocks[k]}:: k in store.blocks.Keys && store.blocks[k].slot > 0 ==>
+    //         store.blocks[k].parent_root in store.blocks.Keys
+    // }
 
     /**
      *  A store where the slots of parent blocks decrease.
      *
      *  @param  store   A store.
      */
-    predicate isSlotDecreasing(store: Store)
-        requires isClosedUnderParent(store)
-    {
-        forall k :: k in store.blocks.Keys && store.blocks[k].slot > 0 ==>
-            store.blocks[store.blocks[k].parent_root].slot < store.blocks[k].slot
-    }
+    // predicate isSlotDecreasing(store: Store)
+    //     requires isClosedUnderParent(store)
+    // {
+    //     forall k :: k in store.blocks.Keys && store.blocks[k].slot > 0 ==>
+    //         store.blocks[store.blocks[k].parent_root].slot < store.blocks[k].slot
+    // }
 
     /**
      *  A chain of blocks roots is a totally ordered (decreasing, slot-wise)
@@ -134,23 +135,23 @@ module ForkChoiceHelpers {
      *  1. br0 ---> br1 ---> br2 ---> br3 ---> br4 ---> br5 and
      *  2. a. and b.
      */
-    predicate isChain(xr: seq<Root>, store: Store)  
-        decreases xr
-    {
-        |xr| >= 1
-        &&
-        (forall i :: 0 <= i < |xr| ==> xr[i] in store.blocks.Keys)
-        && 
-        store.blocks[xr[|xr| - 1]].slot == 0 
-        && 
-        if |xr| == 1 then 
-            //  last block with slot 0 is assumed to be a chain.
-            true
-        else 
-            store.blocks[xr[0]].parent_root == xr[1] 
-            && store.blocks[xr[0]].slot > store.blocks[xr[1]].slot
-            && isChain(xr[1..], store)
-    }
+    // predicate isChain(xr: seq<Root>, store: Store)  
+    //     decreases xr
+    // {
+    //     |xr| >= 1
+    //     &&
+    //     (forall i :: 0 <= i < |xr| ==> xr[i] in store.blocks.Keys)
+    //     && 
+    //     store.blocks[xr[|xr| - 1]].slot == 0 
+    //     && 
+    //     if |xr| == 1 then 
+    //         //  last block with slot 0 is assumed to be a chain.
+    //         true
+    //     else 
+    //         store.blocks[xr[0]].parent_root == xr[1] 
+    //         && store.blocks[xr[0]].slot > store.blocks[xr[1]].slot
+    //         && isChain(xr[1..], store)
+    // }
 
     /**
      *  The ancestors of a block root, as a sequence of block roots.
@@ -170,27 +171,27 @@ module ForkChoiceHelpers {
      *  block   b5----------->b4---------->b3---->b2------>b1------->b0 == br     
      *  slot    0             32           63     95       109       134
      */
-    function chainRoots(br: Root, store: Store) : seq<Root>
-        /** The block root must in the store.  */
-        requires br in store.blocks.Keys
-        /** Store is well-formed. */
-        requires isClosedUnderParent(store)
-        /**  The decreasing property guarantees that this function terminates. */
-        requires isSlotDecreasing(store)
+    // function chainRoots(br: Root, store: Store) : seq<Root>
+    //     /** The block root must in the store.  */
+    //     requires br in store.blocks.Keys
+    //     /** Store is well-formed. */
+    //     requires isClosedUnderParent(store)
+    //     /**  The decreasing property guarantees that this function terminates. */
+    //     requires isSlotDecreasing(store)
 
-        ensures |chainRoots(br, store)| >= 1  
-        /** Result is a slot-decreasing chain of linked roots the last one is slot 0..  */
-        ensures isChain(chainRoots(br, store), store)
+    //     ensures |chainRoots(br, store)| >= 1  
+    //     /** Result is a slot-decreasing chain of linked roots the last one is slot 0..  */
+    //     ensures isChain(chainRoots(br, store), store)
 
-        //  Computation always terminates as slot number decreases (well-foundedness).
-        decreases store.blocks[br].slot
-    {
-        if ( store.blocks[br].slot == 0 ) then
-            //  Should be the genesis block.
-            [ br ]
-        else 
-            [ br ] + chainRoots(store.blocks[br].parent_root, store)
-    }
+    //     //  Computation always terminates as slot number decreases (well-foundedness).
+    //     decreases store.blocks[br].slot
+    // {
+    //     if ( store.blocks[br].slot == 0 ) then
+    //         //  Should be the genesis block.
+    //         [ br ]
+    //     else 
+    //         [ br ] + chainRoots(store.blocks[br].parent_root, store)
+    // }
 
     /**
      *  The height of a block in the store.
@@ -199,22 +200,22 @@ module ForkChoiceHelpers {
      *  @param  store   A store.
      *  @returns        The height of the block br.
      */
-    function height(br: Root, store: Store): nat 
-        /** The block root must in the store.  */
-        requires br in store.blocks.Keys
-        /** Store is well-formed. */
-        requires isClosedUnderParent(store)
-        /**  The decreasing property guarantees that this function terminates. */
-        requires isSlotDecreasing(store)
+    // function height(br: Root, store: Store): nat 
+    //     /** The block root must in the store.  */
+    //     requires br in store.blocks.Keys
+    //     /** Store is well-formed. */
+    //     requires isClosedUnderParent(store)
+    //     /**  The decreasing property guarantees that this function terminates. */
+    //     requires isSlotDecreasing(store)
 
-         decreases store.blocks[br].slot
-    {
-        if ( store.blocks[br].slot == 0 ) then
-            //  Should be the genesis block.
-            0
-        else 
-            1 + height(store.blocks[br].parent_root, store)
-    }
+    //      decreases store.blocks[br].slot
+    // {
+    //     if ( store.blocks[br].slot == 0 ) then
+    //         //  Should be the genesis block.
+    //         0
+    //     else 
+    //         1 + height(store.blocks[br].parent_root, store)
+    // }
 
     /**
      *  Compute the first block root in chain with slot number less than or equal to an epoch.
